src/examples/mutex/liveness_simpler.v
@@ -1,0 +1,293 @@
+From Coq.Relations Require Import Relation_Operators.
+From Coq.Wellfounded Require Import Lexicographic_Product.
+
+From TLA.examples.mutex Require Import nodup automation safety.
+
+Section example.
+
+Implicit Types (σ: State) (s: Config) (t: Tid) (tp: gmap Tid pc.t).
+Implicit Types (l: bool) (q: list Tid).
+
+Lemma fair_step (tid: nat) :
+  fair ⊢ weak_fairness (step tid).
+Proof.
+  unfold fair.
+  (* apply doesn't work due to the wrong unification heuristics *)
+  refine (forall_apply _ _).
+Qed.
+
+(* specialized wf1 rule that handles some common manipulation for this state
+machine *)
+Lemma mutex_wf1 (t: Tid) (P Q: Config → Prop) :
+  (∀ t' σ tp pc σ' pc',
+     let s := {| state := σ; tp := tp|} in
+     let s' := {| state := σ'; tp := <[t' := pc']> tp |} in
+     ∀ (Hpre: P s)
+       (Hinv: all_invs s)
+       (Hinv': all_invs s')
+       (Hneq: t ≠ t')
+       (Hlookup: tp !! t' = Some pc)
+       (Hstep: thread_step t' (σ, pc) (σ', pc')),
+       P s' ∨ Q s'
+  ) →
+  (∀ σ tp pc σ' pc',
+     let s := {| state := σ; tp := tp|} in
+     let s' := {| state := σ'; tp := <[t := pc']> tp |} in
+     ∀ (Hpre: P s)
+       (Hinv: all_invs s)
+       (Hlookup: tp !! t = Some pc)
+       (Hstep: thread_step t (σ, pc) (σ', pc')),
+     Q s'
+  ) →
+  (∀ l q tp,
+     let s := {| state := {| lock := l; queue := q |}; tp := tp |} in
+     P s →
+     ∃ pc, tp !! t = Some pc ∧
+           (pc = pc.kernel_wait → t ∉ q) ∧
+           pc ≠ pc.finished
+  ) →
+  spec ⊢ ⌜P⌝ ~~> ⌜Q⌝.
+Proof.
+  simpl.
+  intros H1 H2 H3.
+  apply (add_safety all_invs_ok).
+  tla_apply (wf1 (step t)).
+  { rewrite /spec.
+    tla_split; [ tla_assumption | tla_apply fair_step ]. }
+  - intros [σ tp] [σ' tp'].
+    intros Hp Hnext.
+    destruct Hnext as [Hnext [Hinvs Hinvs']].
+    apply next_inv in Hnext as
+        [[[=] ?] |
+          (t' & pc & pc' & Hlookup & Hstep & ?)]; subst; eauto.
+    (* in one branch we use the proof that P ∨ Q is preserved, in the other we
+    use the proof that [step t] leads to Q *)
+    destruct (decide (t = t')); subst; eauto.
+  - intros [σ tp] [σ' tp'].
+    intros Hp [_ [Hinvs Hinvs']] Hstep.
+    destruct Hstep as [pc'' [Hlookup [ρ' [Hstep Heq]]]].
+    invc Heq.
+    destruct ρ' as [σ' tp']; simpl in *.
+    eauto.
+  - intros [[l q] tp] HP.
+    rewrite step_enabled /=.
+    eauto.
+Qed.
+
+Definition measure (s: Config) : gset Tid * gset Tid * gset Tid :=
+  (wait_set s.(tp), pc_set pc.unlock_store s.(tp), pc_set pc.unlock_wake s.(tp)).
+
+Definition h_lt : relation (gset Tid * gset Tid * gset Tid) :=
+  slexprod _ _ (slexprod _ _ (⊂) (⊂)) (⊂).
+
+Infix "≺" := h_lt (at level 70).
+
+Definition h_le : relation (gset Tid * gset Tid * gset Tid) :=
+  λ ss ss', ss = ss' ∨ ss ≺ ss'.
+
+Infix "⪯" := h_le (at level 70).
+
+Lemma unlock_set_lock_inv s :
+  all_invs s →
+  s.(state).(lock) = true →
+  ∃ t, pc_set pc.unlock_store s.(tp) = {[t]} ∧
+       s.(tp) !! t = Some pc.unlock_store.
+Proof.
+  destruct 1; intros Hlock.
+  apply Hlocked in Hlock as [t Hlock].
+  rewrite /lock_held in Hlock.
+  exists t; intuition idtac.
+  cut ({[t]} ⊆ pc_set pc.unlock_store s.(tp) ⊆ {[t]}); [ set_solver | ].
+  split.
+  - apply singleton_subseteq_l.
+    auto.
+  - apply elem_of_subseteq => t'.
+    rewrite elem_pc_set => Hlock'.
+    assert (t = t') by (apply Hexcl; eauto); set_solver.
+Qed.
+
+Lemma unlock_set_unlocked_inv s :
+  all_invs s →
+  pc_set pc.unlock_store s.(tp) = ∅ →
+  s.(state).(lock) = false.
+Proof.
+  intros Hinv Hempty.
+  destruct s.(state).(lock) eqn:Hlock; [ exfalso | done ].
+  apply unlock_set_lock_inv in Hlock as [t Hlock]; intuition idtac.
+  set_solver.
+Qed.
+
+Lemma unlock_set_unlocked_inv' s :
+  all_invs s →
+  s.(state).(lock) = false →
+  pc_set pc.unlock_store s.(tp) = ∅.
+Proof.
+  destruct 1; intros Hlock.
+  apply elem_of_equiv_empty_L => t.
+  rewrite elem_pc_set => Hlock'.
+  apply Hexcl in Hlock'.
+  congruence.
+Qed.
+
+Lemma leads_to_if_lock Γ (P: Config → Prop) φ :
+  (Γ ⊢ ⌜λ s, P s ∧ s.(state).(lock) = false⌝ ~~> φ) →
+  (Γ ⊢ ⌜λ s, P s ∧ s.(state).(lock) = true⌝ ~~> φ) →
+  Γ ⊢ ⌜P⌝ ~~> φ.
+Proof.
+  intros Hfalse Htrue.
+  apply (leads_to_if ⌜λ s, s.(state).(lock) = true⌝); tla_simp; auto.
+  leads_to_etrans; [ | apply Hfalse ].
+  lt_unfold. rewrite not_true_iff_false //.
+Qed.
+
+Hint Constructors slexprod : core.
+
+Lemma measure_lt1 Sₗ Sᵤ S__w Sₗ' Sᵤ' S__w' :
+  Sₗ' ⊂ Sₗ →
+  (Sₗ', Sᵤ', S__w') ≺ (Sₗ, Sᵤ, S__w).
+Proof.
+  rewrite /h_lt. auto.
+Qed.
+
+Lemma measure_lt2 Sₗ Sᵤ S__w Sᵤ' S__w' :
+  Sᵤ' ⊂ Sᵤ →
+  (Sₗ, Sᵤ', S__w') ≺ (Sₗ, Sᵤ, S__w).
+Proof.
+  rewrite /h_lt. auto.
+Qed.
+
+Lemma measure_lt3 Sₗ Sᵤ S__w S__w' :
+  S__w' ⊂ S__w →
+  (Sₗ, Sᵤ, S__w') ≺ (Sₗ, Sᵤ, S__w).
+Proof.
+  rewrite /h_lt. auto.
+Qed.
+
+Hint Resolve measure_lt1 measure_lt2 measure_lt3 : core.
+
+Lemma measure_lt_unfold Sₗ Sᵤ S__w Sₗ' Sᵤ' S__w' :
+  (Sₗ', Sᵤ', S__w') ≺ (Sₗ, Sᵤ, S__w) ↔
+  Sₗ' ⊂ Sₗ ∨
+  (Sₗ' = Sₗ ∧ Sᵤ' ⊂ Sᵤ) ∨
+  (Sₗ' = Sₗ ∧ Sᵤ' = Sᵤ ∧ S__w' ⊂ S__w).
+Proof.
+  split.
+  - intros H; invc H; eauto.
+    invc H1; eauto.
+  - intuition (subst; eauto).
+Qed.
+
+Lemma tuple_eq_unfold (S1 S2 S3 S1' S2' S3': gset Tid) :
+  (S1, S2, S3) = (S1', S2', S3') ↔
+  S1 = S1' ∧ S2 = S2' ∧ S3 = S3'.
+Proof. naive_solver. Qed.
+
+Hint Rewrite tuple_eq_unfold measure_lt_unfold : pc.
+
+Lemma eventually_unlocked ss :
+  spec ⊢ ⌜λ s, measure s = ss⌝ ~~>
+         ⌜λ s, measure s ≺ ss ∨
+               measure s = ss ∧
+               let '(_, Sᵤ', _) := measure s in
+               Sᵤ' = ∅ ∧ s.(state).(lock) = false⌝.
+Proof.
+  apply (leads_to_assume _ all_invs_ok). lt_simp.
+  apply leads_to_if_lock.
+  - lt_unfold.
+    intuition subst.
+    simpl.
+    right; intuition auto.
+    apply unlock_set_unlocked_inv' in H1; auto.
+  - leads_to_trans (∃ t, ⌜λ s, measure s = ss ∧
+                   pc_set pc.unlock_store s.(tp) = {[t]} ∧
+                   s.(tp) !! t = Some pc.unlock_store⌝)%L.
+    { lt_unfold. intuition subst.
+      apply unlock_set_lock_inv in H1 as [t ?]; eauto. }
+    lt_intros.
+    rewrite /measure.
+    apply (mutex_wf1 t); simpl; intros.
+    + destruct ss as [[Sₗ Sᵤ] S__w].
+      destruct_step; stm.
+    + destruct ss as [[Sₗ Sᵤ] S__w].
+      stm.
+    + naive_solver.
+Qed.
+
+Lemma eventually_unlocked2 ss :
+  spec ⊢ ⌜λ s, measure s = ss ⌝ ~~>
+         ⌜λ s, measure s ≺ ss ∨
+               measure s = ss ∧
+               let '(_, Sᵤ', S__w') := measure s in
+               Sᵤ' = ∅ ∧ S__w' = ∅ ∧ s.(state).(lock) = false⌝.
+Proof.
+  leads_to_etrans.
+  { apply eventually_unlocked. }
+  lt_split; [ by lt_auto | ].
+  simpl.
+  destruct ss as [[Sₗ Sᵤ] S__w].
+  destruct (decide (S__w = ∅)); subst.
+  { lt_unfold.
+    rewrite /measure; stm.
+    rewrite H H4; auto. }
+  apply set_choose_L in n as [t Hwake].
+  rewrite /measure.
+  lt_simp.
+  apply (mutex_wf1 t); simpl; intros.
+  - destruct_step; stm.
+  - intuition subst.
+    assert (tp !! t = Some pc.unlock_wake).
+    { stm. apply elem_pc_set in Hwake; auto. }
+    stm.
+  - stm.
+    assert (tp !! t = Some pc.unlock_wake).
+    { stm. apply elem_pc_set in Hwake; auto. }
+    naive_solver.
+Qed.
+
+Lemma eventually_progress_atomic_cas Sₗ t :
+  t ∈ Sₗ →
+  spec ⊢ ⌜λ s, measure s = (Sₗ, ∅, ∅) ∧
+               s.(tp) !! t = Some pc.lock_cas ⌝ ~~>
+         ⌜λ s, measure s ≺ (Sₗ, ∅, ∅)⌝.
+Proof.
+  intros Hel.
+  rewrite /measure.
+  apply (mutex_wf1 t); simpl; intros.
+  - destruct_step; stm.
+    rewrite H4 H3. simp_props.
+    apply elem_pc_set in Hlookup.
+    set_solver.
+  - stm.
+    destruct l0; stm.
+    exfalso.
+    apply unlock_set_lock_inv in Hinv as [t' ?]; intuition.
+    simpl in *.
+    set_solver.
+  - naive_solver.
+Qed.
+
+Lemma eventually_progress_futex_wait Sₗ t :
+  t ∈ Sₗ →
+  spec ⊢ ⌜λ s, measure s = (Sₗ, ∅, ∅) ∧
+               s.(tp) !! t = Some pc.futex_wait ⌝ ~~>
+         ⌜λ s, measure s ≺ (Sₗ, ∅, ∅)⌝.
+Proof.
+  intros Hel.
+  eapply leads_to_detour; [ | apply eventually_progress_atomic_cas; eauto ].
+  lt_simp.
+  rewrite /measure.
+  apply (mutex_wf1 t); simpl; intros.
+  - destruct_step; stm.
+    rewrite H4 H3. simp_props.
+    apply elem_pc_set in Hlookup.
+    set_solver.
+  - stm.
+    destruct l0; stm.
+    exfalso.
+    apply unlock_set_lock_inv in Hinv as [t' ?]; intuition.
+    simpl in *.
+    set_solver.
+  - naive_solver.
+Qed.
+
+End example.
